checkpoing

boogie/sorted-list/sorted-list.bpl
@@ -1,5 +1,10 @@
-// Sorted List Insert
-// Cody Rivera
+// Supporting Artifact for
+// "Predictive Verification using Intrinsic Definitions of Data Structures"
+// by Adithya Murali, Cody Rivera, and P. Madhusudan.
+// 
+// Artifact by Cody Rivera, 2023. 
+//
+// Definition of Sorted Lists.
 
 // Datatype aliases
 type Ref;
@@ -8,184 +13,39 @@ const null: Ref;
 type KeySet = [int]bool;
 type RefSet = [Ref]bool;
 
-// Define necessary set operations and constants.
-
-// Operations and constants for key sets.
+// Set library
 const EmptyKeySet: KeySet;
-
+function KeySetMember(x: int, s2: KeySet) returns (bool);
+function KeySetAddF(s: KeySet, x: int) returns (KeySet);
+function KeySetRemoveF(s: KeySet, x: int) returns (KeySet);
+function KeySetIntersectF(s1: KeySet, s2: KeySet) returns (KeySet);
 function KeySetUnionF(s1: KeySet, s2: KeySet) returns (KeySet);
-
+function KeySetComF(s: KeySet) returns (KeySet);
 function KeySetDiffF(s1: KeySet, s2: KeySet) returns (KeySet);
-
+function KeySetSubset(s1: KeySet, s2: KeySet) returns (bool);
 function KeySetsEqual(s1: KeySet, s2: KeySet) returns (bool);
-
 function KeySetsDisjoint(s1: KeySet, s2: KeySet) returns (bool);
 
-// Operations and constants for reference sets.
 const EmptyRefSet: RefSet;
-
+function RefSetMember(x: Ref, s2: RefSet) returns (bool);
+function RefSetAddF(s: RefSet, x: Ref) returns (RefSet);
+function RefSetRemoveF(s: RefSet, x: Ref) returns (RefSet);
+function RefSetIntersectF(s1: RefSet, s2: RefSet) returns (RefSet);
 function RefSetUnionF(s1: RefSet, s2: RefSet) returns (RefSet);
-
+function RefSetComF(s: RefSet) returns (RefSet);
 function RefSetDiffF(s1: RefSet, s2: RefSet) returns (RefSet);
-
 function RefSetSubset(s1: RefSet, s2: RefSet) returns (bool);
-
 function RefSetsEqual(s1: RefSet, s2: RefSet) returns (bool);
-
 function RefSetsDisjoint(s1: RefSet, s2: RefSet) returns (bool);
 
-// Frame Reasoning
-function Frame_k(mod_set: RefSet, old_k: [Ref]int, k: [Ref]int) returns ([Ref]int);
-
-// axiom (forall mod_set: RefSet, old_k: [Ref]int, k: [Ref]int, o: Ref ::
-//     { Frame_k(mod_set, old_k, k)[o] }
-//     Frame_k(mod_set, old_k, k)[o] == (if !mod_set[o] then old_k[o] else k[o]));
-
-function Frame_next(mod_set: RefSet, old_next: [Ref]Ref, next: [Ref]Ref) returns ([Ref]Ref);
-
-// axiom (forall mod_set: RefSet, old_next: [Ref]Ref, next: [Ref]Ref, o: Ref ::
-//     { Frame_next(mod_set, old_next, next)[o] }
-//     Frame_next(mod_set, old_next, next)[o] == (if !mod_set[o] then old_next[o] else next[o]));
-
-function Frame_prev(mod_set: RefSet, old_prev: [Ref]Ref, prev: [Ref]Ref) returns ([Ref]Ref);
-
-// axiom (forall mod_set: RefSet, old_prev: [Ref]Ref, prev: [Ref]Ref, o: Ref ::
-//     { Frame_prev(mod_set, old_prev, prev)[o] }
-//     Frame_prev(mod_set, old_prev, prev)[o] == (if !mod_set[o] then old_prev[o] else prev[o]));
-
-function Frame_keys(mod_set: RefSet, old_keys: [Ref]KeySet, keys: [Ref]KeySet) returns ([Ref]KeySet);
-
-// axiom (forall mod_set: RefSet, old_keys: [Ref]KeySet, keys: [Ref]KeySet, o: Ref ::
-//     { Frame_keys(mod_set, old_keys, keys)[o] }
-//     Frame_keys(mod_set, old_keys, keys)[o] == (if !mod_set[o] then old_keys[o] else keys[o]));
-
-function Frame_repr(mod_set: RefSet, old_repr: [Ref]RefSet, repr: [Ref]RefSet) returns ([Ref]RefSet);
-
-// axiom (forall mod_set: RefSet, old_repr: [Ref]RefSet, repr: [Ref]RefSet, o: Ref ::
-//     { Frame_repr(mod_set, old_repr, repr)[o] }
-//     Frame_repr(mod_set, old_repr, repr)[o] == (if !mod_set[o] then old_repr[o] else repr[o]));
-
-function Frame_sorted(mod_set: RefSet, old_sorted: [Ref]bool, sorted: [Ref]bool) returns ([Ref]bool);
-
-// axiom (forall mod_set: RefSet, old_sorted: [Ref]bool, sorted: [Ref]bool, o: Ref ::
-//     { Frame_sorted(mod_set, old_sorted, sorted)[o] }
-//     Frame_sorted(mod_set, old_sorted, sorted)[o] == (if !mod_set[o] then old_sorted[o] else sorted[o]));
-
-// Alloc set reasoning:
-function {:inline} InAlloc(
-    k: [Ref]int, 
-    next: [Ref]Ref,
-    prev: [Ref]Ref,
-    keys: [Ref]KeySet,
-    repr: [Ref]RefSet,
-    sorted: [Ref]bool,
-    x: Ref,
-    alloc: RefSet
-) returns (bool)
-{
-  x != null ==> (
-    alloc[x]
-    && (next[x] != null ==> alloc[next[x]])
-    && (prev[x] != null ==> alloc[prev[x]])
-    && RefSetSubset(repr[x], alloc)
-  )
-}
-
-// // Axioms for quick checking -- I can easily comment these.
-// // Operations and constants for key sets.
-// axiom (forall o: int :: { EmptyKeySet[o] } !EmptyKeySet[o]);
-
-// axiom (forall a: KeySet, b: KeySet, o: int :: 
-//   { KeySetUnionF(a, b)[o] } 
-//   KeySetUnionF(a, b)[o] <==> a[o] || b[o]);
-
-// axiom (forall a: KeySet, b: KeySet, y: int :: 
-//   { KeySetUnionF(a, b), a[y] } 
-//   a[y] ==> KeySetUnionF(a, b)[y]);
-
-// axiom (forall a: KeySet, b: KeySet, y: int :: 
-//   { KeySetUnionF(a, b), b[y] } 
-//   b[y] ==> KeySetUnionF(a, b)[y]);
-
-// axiom (forall a: KeySet, b: KeySet :: 
-//   { KeySetUnionF(a, b) } 
-//   KeySetsDisjoint(a, b)
-//      ==> KeySetsEqual(KeySetDiffF(KeySetUnionF(a, b), a), b)
-//        && KeySetsEqual(KeySetDiffF(KeySetUnionF(a, b), b), a));
-
-// axiom (forall a: KeySet, b: KeySet, o: int ::
-//   { KeySetDiffF(a, b)[o] } 
-//   KeySetDiffF(a, b)[o] <==> a[o] && !b[o]);
-
-// axiom (forall a: KeySet, b: KeySet, y: int ::
-//   { KeySetDiffF(a, b), b[y] } 
-//   b[y] ==> !KeySetDiffF(a, b)[y]);
-
-// axiom (forall a: KeySet, b: KeySet :: 
-//   { KeySetsEqual(a, b) } 
-//   KeySetsEqual(a, b) <==> (forall o: int :: { a[o] } { b[o] } a[o] <==> b[o]));
-
-// axiom (forall a: KeySet, b: KeySet :: 
-//   { KeySetsEqual(a, b) } 
-//   KeySetsEqual(a, b) ==> a == b);
-
-// axiom (forall a: KeySet, b: KeySet :: 
-//   { KeySetsDisjoint(a, b) } 
-//   KeySetsDisjoint(a, b) <==> (forall o: int :: { a[o] } { b[o] } !a[o] || !b[o]));
-
-// // Operations and constants for reference sets.
-// axiom (forall o: Ref :: { EmptyRefSet[o] } !EmptyRefSet[o]);
-
-// axiom (forall a: RefSet, b: RefSet, o: Ref :: 
-//   { RefSetUnionF(a, b)[o] } 
-//   RefSetUnionF(a, b)[o] <==> a[o] || b[o]);
-
-// axiom (forall a: RefSet, b: RefSet, y: Ref :: 
-//   { RefSetUnionF(a, b), a[y] } 
-//   a[y] ==> RefSetUnionF(a, b)[y]);
-
-// axiom (forall a: RefSet, b: RefSet, y: Ref :: 
-//   { RefSetUnionF(a, b), b[y] } 
-//   b[y] ==> RefSetUnionF(a, b)[y]);
-
-// axiom (forall a: RefSet, b: RefSet :: 
-//   { RefSetUnionF(a, b) } 
-//   RefSetsDisjoint(a, b)
-//      ==> RefSetsEqual(RefSetDiffF(RefSetUnionF(a, b), a), b)
-//        && RefSetsEqual(RefSetDiffF(RefSetUnionF(a, b), b), a));
-
-// axiom (forall a: RefSet, b: RefSet, o: Ref ::
-//   { RefSetDiffF(a, b)[o] } 
-//   RefSetDiffF(a, b)[o] <==> a[o] && !b[o]);
-
-// axiom (forall a: RefSet, b: RefSet, y: Ref ::
-//   { RefSetDiffF(a, b), b[y] } 
-//   b[y] ==> !RefSetDiffF(a, b)[y]);
-
-// axiom (forall a: RefSet, b: RefSet :: 
-//   { RefSetSubset(a, b) } 
-//   RefSetSubset(a, b) <==> (forall o: Ref :: { a[o] } { b[o] } a[o] ==> b[o]));
-
-// axiom (forall a: RefSet, b: RefSet :: 
-//   { RefSetsEqual(a, b) } 
-//   RefSetsEqual(a, b) <==> (forall o: Ref :: { a[o] } { b[o] } a[o] <==> b[o]));
-
-// axiom (forall a: RefSet, b: RefSet :: 
-//   { RefSetsEqual(a, b) } 
-//   RefSetsEqual(a, b) ==> a == b);
-
-// axiom (forall a: RefSet, b: RefSet :: 
-//   { RefSetsDisjoint(a, b) } 
-//   RefSetsDisjoint(a, b) <==> (forall o: Ref :: { a[o] } { b[o] } !a[o] || !b[o]));
-
-
-// Define fields
+// Fields
 var C.k: [Ref]int;
 var C.next: [Ref]Ref;
 var C.prev: [Ref]Ref;
 var C.keys: [Ref]KeySet;
 var C.repr: [Ref]RefSet;
 var C.sorted: [Ref]bool;
+var C.rev_sorted: [Ref]bool;
 
 var Br: RefSet;
 var alloc: RefSet;
@@ -198,7 +58,9 @@ function {:inline} LC(
     keys: [Ref]KeySet,
     repr: [Ref]RefSet,
     sorted: [Ref]bool,
-    x: Ref
+    rev_sorted: [Ref]bool,
+    x: Ref,
+    alloc: RefSet
 ) returns (bool)
 {
     x != null ==> (
@@ -215,8 +77,12 @@ function {:inline} LC(
                 && RefSetsEqual(repr[x], (repr[next[x]])[x := true])
                 && prev[next[x]] == x
                 && (sorted[x] ==> k[x] <= k[next[x]])
-                && sorted[x] == sorted[next[x]])
+                && (rev_sorted[x] ==> k[x] >= k[next[x]])
+                && sorted[x] == sorted[next[x]]
+                && rev_sorted[x] == rev_sorted[next[x]])
+        && !(sorted[x] && rev_sorted[x])
     )
+    && InAlloc(k, next, prev, keys, repr, sorted, rev_sorted, x, alloc)
 }
 
 // Manipulation Macros
@@ -231,55 +97,143 @@ procedure Create(k: int) returns (node: Ref);
     ensures Br == old(Br)[node := true];
 
 procedure Set_k(x: Ref, k: int);
+    requires x != null;
     modifies Br, C.k;
     ensures C.k == old(C.k)[x := k];
     ensures C.prev[x] != null ==> Br == (old(Br)[x := true])[C.prev[x] := true];
     ensures C.prev[x] == null ==> Br == old(Br)[x := true];
 
 procedure Set_next(x: Ref, next: Ref);
+    requires x != null;
     modifies Br, C.next;
     ensures C.next == old(C.next)[x := next];
     ensures old(C.next)[x] != null ==> Br == (old(Br)[x := true])[old(C.next)[x] := true];
     ensures old(C.next)[x] == null ==> Br == old(Br)[x := true];
 
 procedure Set_prev(x: Ref, prev: Ref);
+    requires x != null;
     modifies Br, C.prev;
     ensures C.prev == old(C.prev)[x := prev];
     ensures old(C.prev)[x] != null ==> Br == (old(Br)[x := true])[old(C.prev)[x] := true];
     ensures old(C.prev)[x] == null ==> Br == old(Br)[x := true];
 
 procedure Set_keys(x: Ref, keys: KeySet);
+    requires x != null;
     modifies Br, C.keys;
     ensures C.keys == old(C.keys)[x := keys];
     ensures C.prev[x] != null ==> Br == (old(Br)[x := true])[C.prev[x] := true];
     ensures C.prev[x] == null ==> Br == old(Br)[x := true];
 
 procedure Set_repr(x: Ref, repr: RefSet);
+    requires x != null;
     modifies Br, C.repr;
     ensures C.repr == old(C.repr)[x := repr];
     ensures C.prev[x] != null ==> Br == (old(Br)[x := true])[C.prev[x] := true];
     ensures C.prev[x] == null ==> Br == old(Br)[x := true];
 
 procedure Set_sorted(x: Ref, sorted: bool);
+    requires x != null;
     modifies Br, C.sorted;
     ensures C.sorted == old(C.sorted)[x := sorted];
     ensures C.prev[x] != null ==> Br == (old(Br)[x := true])[C.prev[x] := true];
     ensures C.prev[x] == null ==> Br == old(Br)[x := true];
 
+procedure Set_rev_sorted(x: Ref, rev_sorted: bool);
+    requires x != null;
+    modifies Br, C.rev_sorted;
+    ensures C.rev_sorted == old(C.rev_sorted)[x := rev_sorted];
+    ensures C.prev[x] != null ==> Br == (old(Br)[x := true])[C.prev[x] := true];
+    ensures C.prev[x] == null ==> Br == old(Br)[x := true];
+
 // Broken Set Manipulation
 procedure IfNotBr_ThenLC(x: Ref);
-    ensures x != null && !Br[x] ==> LC(C.k, C.next, C.prev, C.keys, C.repr, C.sorted, x);
+    ensures x != null && !Br[x] ==> LC(C.k, C.next, C.prev, C.keys, C.repr, C.sorted, C.rev_sorted, x, alloc);
 
 procedure AssertLCAndRemove(x: Ref);
     modifies Br;
-    ensures (x != null && LC(C.k, C.next, C.prev, C.keys, C.repr, C.sorted, x)) 
+    ensures (x != null && LC(C.k, C.next, C.prev, C.keys, C.repr, C.sorted, C.rev_sorted, x, alloc)) 
                 ==> Br == old(Br)[x := false];
-    ensures (x == null || !LC(C.k, C.next, C.prev, C.keys, C.repr, C.sorted, x))
+    ensures (x == null || !LC(C.k, C.next, C.prev, C.keys, C.repr, C.sorted, C.rev_sorted, x, alloc))
                 ==> Br == old(Br);
 
-function {:inline} fresh(expr: RefSet, newalloc: RefSet, oldalloc: RefSet) returns (bool)
+// Framing
+function Frame_k(mod_set: RefSet, old_k: [Ref]int, k: [Ref]int) returns ([Ref]int);
+function Frame_next(mod_set: RefSet, old_next: [Ref]Ref, next: [Ref]Ref) returns ([Ref]Ref);
+function Frame_prev(mod_set: RefSet, old_prev: [Ref]Ref, prev: [Ref]Ref) returns ([Ref]Ref);
+function Frame_keys(mod_set: RefSet, old_keys: [Ref]KeySet, keys: [Ref]KeySet) returns ([Ref]KeySet);
+function Frame_repr(mod_set: RefSet, old_repr: [Ref]RefSet, repr: [Ref]RefSet) returns ([Ref]RefSet);
+function Frame_sorted(mod_set: RefSet, old_sorted: [Ref]bool, sorted: [Ref]bool) returns ([Ref]bool);
+function Frame_rev_sorted(mod_set: RefSet, old_rev_sorted: [Ref]bool, rev_sorted: [Ref]bool) returns ([Ref]bool);
+
+function {:inline} Frame_all(
+    k: [Ref]int, 
+    next: [Ref]Ref,
+    prev: [Ref]Ref,
+    keys: [Ref]KeySet,
+    repr: [Ref]RefSet,
+    sorted: [Ref]bool,
+    rev_sorted: [Ref]bool,
+    oldk: [Ref]int, 
+    oldnext: [Ref]Ref,
+    oldprev: [Ref]Ref,
+    oldkeys: [Ref]KeySet,
+    oldrepr: [Ref]RefSet,
+    oldsorted: [Ref]bool,
+    oldrev_sorted: [Ref]bool,
+    mod_set: RefSet,
+    old_alloc: RefSet
+) returns (bool) 
+{
+    k == Frame_k(RefSetUnionF(mod_set, RefSetComF(old_alloc)), oldk, k) 
+    && next == Frame_next(RefSetUnionF(mod_set, RefSetComF(old_alloc)), oldnext, next) 
+    && prev == Frame_prev(RefSetUnionF(mod_set, RefSetComF(old_alloc)), oldprev, prev)
+    && keys == Frame_keys(RefSetUnionF(mod_set, RefSetComF(old_alloc)), oldkeys, keys)
+    && repr == Frame_repr(RefSetUnionF(mod_set, RefSetComF(old_alloc)), oldrepr, repr)
+    && sorted == Frame_sorted(RefSetUnionF(mod_set, RefSetComF(old_alloc)), oldsorted, sorted)
+    && rev_sorted == Frame_rev_sorted(RefSetUnionF(mod_set, RefSetComF(old_alloc)), oldrev_sorted, rev_sorted)
+}
+
+// Alloc set reasoning
+function {:inline} InAlloc(
+    k: [Ref]int, 
+    next: [Ref]Ref,
+    prev: [Ref]Ref,
+    keys: [Ref]KeySet,
+    repr: [Ref]RefSet,
+    sorted: [Ref]bool,
+    rev_sorted: [Ref]bool,
+    x: Ref,
+    alloc: RefSet
+) returns (bool)
+{
+  x != null ==> (
+    alloc[x]
+    && (next[x] != null ==> alloc[next[x]])
+    && (prev[x] != null ==> alloc[prev[x]])
+    && RefSetSubset(repr[x], alloc)
+  )
+}
+
+function {:inline} Fresh(expr: RefSet, newalloc: RefSet, oldalloc: RefSet) returns (bool)
 {
     RefSetSubset(expr, newalloc)
     && RefSetsDisjoint(expr, oldalloc)
-    && RefSetSubset(oldalloc, newalloc) // try to see if can be rewritten elsewhere
+}
+
+// Auxiliary functions
+function {:inline} Isolated(
+    k: [Ref]int, 
+    next: [Ref]Ref,
+    prev: [Ref]Ref,
+    keys: [Ref]KeySet,
+    repr: [Ref]RefSet,
+    sorted: [Ref]bool,
+    rev_sorted: [Ref]bool,
+    x: Ref
+) returns (bool)
+{
+  x != null ==> (
+    next[x] == null
+    && prev[x] == null
+  )
 }
