boogie/red-black-tree/red-black-tree.bpl
@@ -1,0 +1,466 @@
+// Supporting Artifact for
+// "Predictive Verification using Intrinsic Definitions of Data Structures"
+// by Adithya Murali, Cody Rivera, and P. Madhusudan.
+// 
+// Artifact by Cody Rivera, 2023. 
+//
+// Definition of Red-Black Trees.
+
+// Datatype aliases
+type Ref;
+const null: Ref;
+
+type KeySet = [int]bool;
+type RefSet = [Ref]bool;
+
+// Set library
+const EmptyKeySet: KeySet;
+function KeySetMember(x: int, s2: KeySet) returns (bool);
+function KeySetAddF(s: KeySet, x: int) returns (KeySet);
+function KeySetRemoveF(s: KeySet, x: int) returns (KeySet);
+function KeySetIntersectF(s1: KeySet, s2: KeySet) returns (KeySet);
+function KeySetUnionF(s1: KeySet, s2: KeySet) returns (KeySet);
+function KeySetComF(s: KeySet) returns (KeySet);
+function KeySetDiffF(s1: KeySet, s2: KeySet) returns (KeySet);
+function KeySetSubset(s1: KeySet, s2: KeySet) returns (bool);
+function KeySetsEqual(s1: KeySet, s2: KeySet) returns (bool);
+function KeySetsDisjoint(s1: KeySet, s2: KeySet) returns (bool);
+
+const EmptyRefSet: RefSet;
+function RefSetMember(x: Ref, s2: RefSet) returns (bool);
+function RefSetAddF(s: RefSet, x: Ref) returns (RefSet);
+function RefSetRemoveF(s: RefSet, x: Ref) returns (RefSet);
+function RefSetIntersectF(s1: RefSet, s2: RefSet) returns (RefSet);
+function RefSetUnionF(s1: RefSet, s2: RefSet) returns (RefSet);
+function RefSetComF(s: RefSet) returns (RefSet);
+function RefSetDiffF(s1: RefSet, s2: RefSet) returns (RefSet);
+function RefSetSubset(s1: RefSet, s2: RefSet) returns (bool);
+function RefSetsEqual(s1: RefSet, s2: RefSet) returns (bool);
+function RefSetsDisjoint(s1: RefSet, s2: RefSet) returns (bool);
+
+// Fields
+var C.k: [Ref]int;
+var C.l: [Ref]Ref;
+var C.r: [Ref]Ref;
+var C.p: [Ref]Ref;
+var C.min: [Ref]int;
+var C.max: [Ref]int;
+var C.keys: [Ref]KeySet;
+var C.repr: [Ref]RefSet;
+var C.black: [Ref]bool;
+var C.black_height: [Ref]int;
+
+var Br: RefSet;
+var alloc: RefSet;
+
+// Local conditions
+function {:inline} LC(
+    k: [Ref]int, 
+    l: [Ref]Ref,
+    r: [Ref]Ref,
+    p: [Ref]Ref,
+    min: [Ref]int,
+    max: [Ref]int,
+    keys: [Ref]KeySet,
+    repr: [Ref]RefSet,
+    black: [Ref]bool,
+    black_height: [Ref]int,
+    x: Ref,
+    alloc: RefSet
+) returns (bool)
+{
+    x != null ==> (
+        (repr[x])[x]
+        && min[x] <= k[x] 
+        && k[x] <= max[x]
+        && (p[x] != null ==>
+                !(repr[x])[p[x]]
+                && (l[p[x]] == x || r[p[x]] == x))
+        && (l[x] != null ==> 
+                (repr[x])[l[x]]
+                && !(repr[l[x]])[x]
+                && p[l[x]] == x
+                && max[l[x]] < k[x])
+        && (r[x] != null ==> 
+                (repr[x])[r[x]]
+                && !(repr[r[x]])[x]
+                && p[r[x]] == x
+                && min[r[x]] > k[x])
+        && (l[x] == null && r[x] == null ==>
+                RefSetsEqual(repr[x], EmptyRefSet[x := true])
+                && KeySetsEqual(keys[x], EmptyKeySet[k[x] := true])
+                && min[x] == k[x] 
+                && k[x] == max[x]
+                )
+        && (l[x] != null && r[x] == null ==>
+                RefSetsEqual(repr[x], (repr[l[x]])[x := true])
+                && KeySetsEqual(keys[x], (keys[l[x]])[k[x] := true])
+                && !(keys[l[x]])[k[x]]
+                && min[x] == min[l[x]] && max[x] == k[x]
+                )
+        && (l[x] == null && r[x] != null ==>
+                RefSetsEqual(repr[x], (repr[r[x]])[x := true])
+                && KeySetsEqual(keys[x], (keys[r[x]])[k[x] := true])
+                && !(keys[r[x]])[k[x]]
+                && min[x] == k[x] && max[x] == max[r[x]]
+                )
+        && (l[x] != null && r[x] != null ==>
+                RefSetsEqual(repr[x], RefSetUnionF((repr[l[x]])[x := true], repr[r[x]]))
+                && RefSetsDisjoint(repr[l[x]], repr[r[x]])
+                && KeySetsEqual(keys[x], KeySetUnionF((keys[l[x]])[k[x] := true], keys[r[x]]))
+                && KeySetsDisjoint(keys[l[x]], keys[r[x]])
+                && !(keys[l[x]])[k[x]] && !(keys[r[x]])[k[x]]
+                && min[x] == min[l[x]] && max[x] == max[r[x]]
+                )
+        // Special RBT properties
+        && (l[x] == null && r[x] == null ==>
+                black_height[x] == (if black[x] then 1 else 0))
+        && (l[x] != null && r[x] == null ==>
+                black_height[x] == (if black[x] then 1 else 0)
+                && black_height[l[x]] == 0
+                && (black[x] || black[l[x]]))
+        && (l[x] == null && r[x] != null ==>
+                black_height[x] == (if black[x] then 1 else 0)
+                && black_height[r[x]] == 0
+                && (black[x] || black[r[x]]))
+        && (l[x] != null && r[x] != null ==>
+                (black_height[l[x]] > black_height[r[x]] ==>
+                    black_height[x] == (if black[x] then black_height[l[x]] + 1 else black_height[l[x]]))
+                && (black_height[l[x]] <= black_height[r[x]] ==>
+                        black_height[x] == (if black[x] then black_height[r[x]] + 1 else black_height[r[x]]))
+                && black_height[l[x]] == black_height[r[x]]
+                && (black[x] || (black[l[x]] && black[r[x]])))
+    )
+    && InAlloc(k, l, r, p, min, max,
+               keys, repr, black, black_height, x, alloc)
+}
+
+function {:inline} LC_Trans_RedRed(
+    k: [Ref]int, 
+    l: [Ref]Ref,
+    r: [Ref]Ref,
+    p: [Ref]Ref,
+    min: [Ref]int,
+    max: [Ref]int,
+    keys: [Ref]KeySet,
+    repr: [Ref]RefSet,
+    black: [Ref]bool,
+    black_height: [Ref]int,
+    x: Ref,
+    alloc: RefSet
+) returns (bool)
+{
+    x != null ==> (
+        (repr[x])[x]
+        && min[x] <= k[x] 
+        && k[x] <= max[x]
+        && (p[x] != null ==>
+                !(repr[x])[p[x]]
+                && (l[p[x]] == x || r[p[x]] == x))
+        && (l[x] != null ==> 
+                (repr[x])[l[x]]
+                && !(repr[l[x]])[x]
+                && p[l[x]] == x
+                && max[l[x]] < k[x])
+        && (r[x] != null ==> 
+                (repr[x])[r[x]]
+                && !(repr[r[x]])[x]
+                && p[r[x]] == x
+                && min[r[x]] > k[x])
+        && (l[x] == null && r[x] == null ==>
+                RefSetsEqual(repr[x], EmptyRefSet[x := true])
+                && KeySetsEqual(keys[x], EmptyKeySet[k[x] := true])
+                && min[x] == k[x] 
+                && k[x] == max[x]
+                )
+        && (l[x] != null && r[x] == null ==>
+                RefSetsEqual(repr[x], (repr[l[x]])[x := true])
+                && KeySetsEqual(keys[x], (keys[l[x]])[k[x] := true])
+                && !(keys[l[x]])[k[x]]
+                && min[x] == min[l[x]] && max[x] == k[x]
+                )
+        && (l[x] == null && r[x] != null ==>
+                RefSetsEqual(repr[x], (repr[r[x]])[x := true])
+                && KeySetsEqual(keys[x], (keys[r[x]])[k[x] := true])
+                && !(keys[r[x]])[k[x]]
+                && min[x] == k[x] && max[x] == max[r[x]]
+                )
+        && (l[x] != null && r[x] != null ==>
+                RefSetsEqual(repr[x], RefSetUnionF((repr[l[x]])[x := true], repr[r[x]]))
+                && RefSetsDisjoint(repr[l[x]], repr[r[x]])
+                && KeySetsEqual(keys[x], KeySetUnionF((keys[l[x]])[k[x] := true], keys[r[x]]))
+                && KeySetsDisjoint(keys[l[x]], keys[r[x]])
+                && !(keys[l[x]])[k[x]] && !(keys[r[x]])[k[x]]
+                && min[x] == min[l[x]] && max[x] == max[r[x]]
+                )
+        // Special RBT properties
+        && (l[x] == null && r[x] == null ==>
+                black_height[x] == (if black[x] then 1 else 0))
+        && (l[x] != null && r[x] == null ==>
+                black_height[x] == (if black[x] then 1 else 0)
+                && black_height[l[x]] == 0)
+        && (l[x] == null && r[x] != null ==>
+                black_height[x] == (if black[x] then 1 else 0)
+                && black_height[r[x]] == 0)
+        && (l[x] != null && r[x] != null ==>
+                (black_height[l[x]] > black_height[r[x]] ==>
+                    black_height[x] == (if black[x] then black_height[l[x]] + 1 else black_height[l[x]]))
+                && (black_height[l[x]] <= black_height[r[x]] ==>
+                        black_height[x] == (if black[x] then black_height[r[x]] + 1 else black_height[r[x]]))
+                && black_height[l[x]] == black_height[r[x]])
+        && black_height[x] >= 0
+    )
+    && InAlloc(k, l, r, p, min, max,
+               keys, repr, black, black_height, x, alloc)
+}
+
+function {:inline} LC_Trans_DoubleBlack(
+    k: [Ref]int, 
+    l: [Ref]Ref,
+    r: [Ref]Ref,
+    p: [Ref]Ref,
+    min: [Ref]int,
+    max: [Ref]int,
+    keys: [Ref]KeySet,
+    repr: [Ref]RefSet,
+    black: [Ref]bool,
+    black_height: [Ref]int,
+    x: Ref,
+    alloc: RefSet
+) returns (bool)
+{
+    x != null ==> (
+        (repr[x])[x]
+        && min[x] <= k[x] 
+        && k[x] <= max[x]
+        && (p[x] != null ==>
+                !(repr[x])[p[x]]
+                && (l[p[x]] == x || r[p[x]] == x))
+        && (l[x] != null ==> 
+                (repr[x])[l[x]]
+                && !(repr[l[x]])[x]
+                && p[l[x]] == x
+                && max[l[x]] < k[x])
+        && (r[x] != null ==> 
+                (repr[x])[r[x]]
+                && !(repr[r[x]])[x]
+                && p[r[x]] == x
+                && min[r[x]] > k[x])
+        && (l[x] == null && r[x] == null ==>
+                RefSetsEqual(repr[x], EmptyRefSet[x := true])
+                && KeySetsEqual(keys[x], EmptyKeySet[k[x] := true])
+                && min[x] == k[x] 
+                && k[x] == max[x]
+                )
+        && (l[x] != null && r[x] == null ==>
+                RefSetsEqual(repr[x], (repr[l[x]])[x := true])
+                && KeySetsEqual(keys[x], (keys[l[x]])[k[x] := true])
+                && !(keys[l[x]])[k[x]]
+                && min[x] == min[l[x]] && max[x] == k[x]
+                )
+        && (l[x] == null && r[x] != null ==>
+                RefSetsEqual(repr[x], (repr[r[x]])[x := true])
+                && KeySetsEqual(keys[x], (keys[r[x]])[k[x] := true])
+                && !(keys[r[x]])[k[x]]
+                && min[x] == k[x] && max[x] == max[r[x]]
+                )
+        && (l[x] != null && r[x] != null ==>
+                RefSetsEqual(repr[x], RefSetUnionF((repr[l[x]])[x := true], repr[r[x]]))
+                && RefSetsDisjoint(repr[l[x]], repr[r[x]])
+                && KeySetsEqual(keys[x], KeySetUnionF((keys[l[x]])[k[x] := true], keys[r[x]]))
+                && KeySetsDisjoint(keys[l[x]], keys[r[x]])
+                && !(keys[l[x]])[k[x]] && !(keys[r[x]])[k[x]]
+                && min[x] == min[l[x]] && max[x] == max[r[x]]
+                )
+        // Special RBT properties
+        && (l[x] == null && r[x] == null ==>
+                black_height[x] == (if black[x] then 1 else 0))
+        && (l[x] != null && r[x] == null ==>
+                black_height[x] == (if black[x] then 1 + black_height[l[x]] else black_height[l[x]])
+                && black_height[l[x]] <= 1
+                && (black[x] || black[l[x]]))
+        && (l[x] == null && r[x] != null ==>
+                black_height[x] == (if black[x] then 1 + black_height[r[x]] else black_height[r[x]])
+                && black_height[r[x]] <= 1
+                && (black[x] || black[r[x]]))
+        && (l[x] != null && r[x] != null ==>
+                (black_height[l[x]] > black_height[r[x]] ==>
+                    black_height[x] == (if black[x] then black_height[l[x]] + 1 else black_height[l[x]]))
+                && (black_height[l[x]] <= black_height[r[x]] ==>
+                        black_height[x] == (if black[x] then black_height[r[x]] + 1 else black_height[r[x]]))
+                && (black_height[l[x]] == black_height[r[x]]
+                    || black_height[l[x]] + 1 == black_height[r[x]]
+                    || black_height[l[x]] == black_height[r[x]] + 1)
+                && (black[x] || (black[l[x]] && black[r[x]])))
+        && black_height[x] >= 0
+    )
+    && InAlloc(k, l, r, p, min, max,
+               keys, repr, black, black_height, x, alloc)
+}
+
+// Manipulation macros
+procedure Create(k: int) returns (node: Ref);
+    modifies Br, alloc, C.k, C.l, C.r, C.p;
+    ensures node != null;
+    ensures !old(alloc)[node];
+    ensures alloc == old(alloc)[node := true];
+    ensures C.k == old(C.k)[node := k];
+    ensures C.l == old(C.l)[node := null];
+    ensures C.r == old(C.r)[node := null];
+    ensures C.p == old(C.p)[node := null];
+    ensures Br == old(Br)[node := true];
+
+procedure Set_k(x: Ref, k: int);
+    requires x != null;
+    modifies Br, C.k;
+    ensures C.k == old(C.k)[x := k];
+    ensures C.p[x] != null ==> Br == (old(Br)[x := true])[C.p[x] := true];
+    ensures C.p[x] == null ==> Br == old(Br)[x := true];
+
+procedure Set_l(x: Ref, l: Ref);
+    requires x != null;
+    modifies Br, C.l;
+    ensures C.l == old(C.l)[x := l];
+    ensures old(C.l)[x] != null ==> Br == (old(Br)[x := true])[old(C.l)[x] := true];
+    ensures old(C.l)[x] == null ==> Br == old(Br)[x := true];
+
+procedure Set_r(x: Ref, r: Ref);
+    requires x != null;
+    modifies Br, C.r;
+    ensures C.r == old(C.r)[x := r];
+    ensures old(C.r)[x] != null ==> Br == (old(Br)[x := true])[old(C.r)[x] := true];
+    ensures old(C.r)[x] == null ==> Br == old(Br)[x := true];
+
+procedure Set_p(x: Ref, p: Ref);
+    requires x != null;
+    modifies Br, C.p;
+    ensures C.p == old(C.p)[x := p];
+    ensures old(C.p)[x] != null ==> Br == (old(Br)[x := true])[old(C.p)[x] := true];
+    ensures old(C.p)[x] == null ==> Br == old(Br)[x := true];
+
+procedure Set_min(x: Ref, min: int);
+    requires x != null;
+    modifies Br, C.min;
+    ensures C.min == old(C.min)[x := min];
+    ensures C.p[x] != null ==> Br == (old(Br)[x := true])[C.p[x] := true];
+    ensures C.p[x] == null ==> Br == old(Br)[x := true];
+
+procedure Set_max(x: Ref, max: int);
+    requires x != null;
+    modifies Br, C.max;
+    ensures C.max == old(C.max)[x := max];
+    ensures C.p[x] != null ==> Br == (old(Br)[x := true])[C.p[x] := true];
+    ensures C.p[x] == null ==> Br == old(Br)[x := true];
+
+procedure Set_keys(x: Ref, keys: KeySet);
+    requires x != null;
+    modifies Br, C.keys;
+    ensures C.keys == old(C.keys)[x := keys];
+    ensures C.p[x] != null ==> Br == (old(Br)[x := true])[C.p[x] := true];
+    ensures C.p[x] == null ==> Br == old(Br)[x := true];
+
+procedure Set_repr(x: Ref, repr: RefSet);
+    requires x != null;
+    modifies Br, C.repr;
+    ensures C.repr == old(C.repr)[x := repr];
+    ensures C.p[x] != null ==> Br == (old(Br)[x := true])[C.p[x] := true];
+    ensures C.p[x] == null ==> Br == old(Br)[x := true];
+
+procedure Set_black(x: Ref, black: bool);
+    requires x != null;
+    modifies Br, C.black;
+    ensures C.black == old(C.black)[x := black];
+    ensures C.p[x] != null ==> Br == (old(Br)[x := true])[C.p[x] := true];
+    ensures C.p[x] == null ==> Br == old(Br)[x := true];
+
+procedure Set_black_height(x: Ref, black_height: int);
+    requires x != null;
+    modifies Br, C.black_height;
+    ensures C.black_height == old(C.black_height)[x := black_height];
+    ensures C.p[x] != null ==> Br == (old(Br)[x := true])[C.p[x] := true];
+    ensures C.p[x] == null ==> Br == old(Br)[x := true];
+
+// Broken set manipulation
+procedure IfNotBr_ThenLC(x: Ref);
+    ensures x != null && !Br[x] ==> LC(C.k, C.l, C.r, C.p, 
+                                        C.min, C.max, C.keys,
+                                        C.repr, C.black, C.black_height, 
+                                        x, alloc);
+
+procedure AssertLCAndRemove(x: Ref);
+    modifies Br;
+    ensures (x != null && LC(C.k, C.l, C.r, C.p, 
+                            C.min, C.max, C.keys,
+                            C.repr, C.black, C.black_height, 
+                            x, alloc)) 
+                ==> Br == old(Br)[x := false];
+    ensures (x == null || !LC(C.k, C.l, C.r, C.p, 
+                            C.min, C.max, C.keys,
+                            C.repr, C.black, C.black_height, 
+                            x, alloc))
+                ==> Br == old(Br);
+
+// Framing
+function Frame_k(mod_set: RefSet, old_k: [Ref]int, k: [Ref]int) returns ([Ref]int);
+function Frame_l(mod_set: RefSet, old_l: [Ref]Ref, l: [Ref]Ref) returns ([Ref]Ref);
+function Frame_r(mod_set: RefSet, old_r: [Ref]Ref, r: [Ref]Ref) returns ([Ref]Ref);
+function Frame_p(mod_set: RefSet, old_p: [Ref]Ref, p: [Ref]Ref) returns ([Ref]Ref);
+function Frame_min(mod_set: RefSet, old_min: [Ref]int, min: [Ref]int) returns ([Ref]int);
+function Frame_max(mod_set: RefSet, old_max: [Ref]int, max: [Ref]int) returns ([Ref]int);
+function Frame_keys(mod_set: RefSet, old_keys: [Ref]KeySet, keys: [Ref]KeySet) returns ([Ref]KeySet);
+function Frame_repr(mod_set: RefSet, old_repr: [Ref]RefSet, repr: [Ref]RefSet) returns ([Ref]RefSet);
+function Frame_black(mod_set: RefSet, old_black: [Ref]bool, black: [Ref]bool) returns ([Ref]bool);
+function Frame_black_height(mod_set: RefSet, old_black_height: [Ref]int, black_height: [Ref]int) returns ([Ref]int);
+
+// Alloc set reasoning
+function {:inline} InAlloc(
+    k: [Ref]int, 
+    l: [Ref]Ref,
+    r: [Ref]Ref,
+    p: [Ref]Ref,
+    min: [Ref]int,
+    max: [Ref]int,
+    keys: [Ref]KeySet,
+    repr: [Ref]RefSet,
+    black: [Ref]bool,
+    black_height: [Ref]int,
+    x: Ref,
+    alloc: RefSet
+) returns (bool)
+{
+    x != null ==> (
+        alloc[x]
+        && (l[x] != null ==> alloc[l[x]])
+        && (r[x] != null ==> alloc[r[x]])
+        && (p[x] != null ==> alloc[p[x]])
+        && RefSetSubset(repr[x], alloc)
+    )
+}
+
+function {:inline} Fresh(expr: RefSet, newalloc: RefSet, oldalloc: RefSet) returns (bool)
+{
+    RefSetSubset(expr, newalloc)
+    && RefSetsDisjoint(expr, oldalloc)
+}
+
+// Auxiliary functions
+function {:inline} Isolated(
+    k: [Ref]int, 
+    l: [Ref]Ref,
+    r: [Ref]Ref,
+    p: [Ref]Ref,
+    min: [Ref]int,
+    max: [Ref]int,
+    keys: [Ref]KeySet,
+    repr: [Ref]RefSet,
+    black: [Ref]bool,
+    black_height: [Ref]int,
+    x: Ref
+) returns (bool)
+{
+  x != null ==> (
+    l[x] == null
+    && r[x] == null
+    && p[x] == null
+  )
+}
