boogie/sorted-list/insert.bpl
@@ -1,53 +1,64 @@
+// Supporting Artifact for
+// "Predictive Verification using Intrinsic Definitions of Data Structures"
+// by Adithya Murali, Cody Rivera, and P. Madhusudan.
+// 
+// Artifact by Cody Rivera, 2023. 
+//
+// Verification of Sorted List Insert.
+
 procedure SortedListInsertContract(x: Ref, k: int) returns (ret: Ref);
     requires RefSetsEqual(Br, EmptyRefSet);
-    requires LC(C.k, C.next, C.prev, C.keys, C.repr, C.sorted, x);
+    requires LC(C.k, C.next, C.prev, C.keys, C.repr, C.sorted, C.rev_sorted, x, alloc);
     requires x != null ==> C.sorted[x];
-    modifies Br, alloc, C.k, C.next, C.prev, C.keys, C.repr, C.sorted;
+    modifies Br, alloc, C.k, C.next, C.prev, C.keys, C.repr, C.sorted, C.rev_sorted;
+    ensures RefSetSubset(old(alloc), alloc);
     ensures ret != null;
-    ensures LC(C.k, C.next, C.prev, C.keys, C.repr, C.sorted, ret);
+    ensures LC(C.k, C.next, C.prev, C.keys, C.repr, C.sorted, C.rev_sorted, ret, alloc);
     ensures C.sorted[ret];
     ensures C.k[ret] == (if x != null && old(C.k)[x] <= k then old(C.k)[x] else k);
     ensures KeySetsEqual(C.keys[ret], (if x == null then EmptyKeySet else old(C.keys)[x])[k := true]);
-    ensures fresh(RefSetDiffF(C.repr[ret], (if x == null then EmptyRefSet else old(C.repr)[x])), alloc, old(alloc));
+    ensures Fresh(RefSetDiffF(C.repr[ret], (if x == null then EmptyRefSet else old(C.repr)[x])), alloc, old(alloc));
     ensures C.prev[ret] == null;
     ensures x != null ==> (ret == x || C.next[ret] == x);
     ensures (x == null || old(C.prev)[x] == null) ==> RefSetsEqual(Br, EmptyRefSet);
     ensures (x != null && old(C.prev)[x] != null) ==> RefSetsEqual(Br, EmptyRefSet[old(C.prev)[x] := true]);
     // Framing conditions.
-    ensures C.k == Frame_k(if x == null then EmptyRefSet else old(C.repr)[x] , old(C.k), C.k);
-    ensures C.next == Frame_next(if x == null then EmptyRefSet else old(C.repr)[x] , old(C.next), C.next);
-    ensures C.prev == Frame_prev(if x == null then EmptyRefSet else old(C.repr)[x] , old(C.prev), C.prev);
-    ensures C.keys == Frame_keys(if x == null then EmptyRefSet else old(C.repr)[x] , old(C.keys), C.keys);
-    ensures C.repr == Frame_repr(if x == null then EmptyRefSet else old(C.repr)[x] , old(C.repr), C.repr);
-    ensures C.sorted == Frame_sorted(if x == null then EmptyRefSet else old(C.repr)[x] , old(C.sorted), C.sorted);
+    ensures Frame_all(C.k, C.next, C.prev, C.keys, C.repr, C.sorted, C.rev_sorted,
+                      old(C.k), old(C.next), old(C.prev), old(C.keys), old(C.repr), old(C.sorted), old(C.rev_sorted),
+                      if x == null then EmptyRefSet else old(C.repr)[x], old(alloc));
 
 procedure SortedListInsert(x: Ref, k: int) returns (ret: Ref)
     requires RefSetsEqual(Br, EmptyRefSet);
-    requires LC(C.k, C.next, C.prev, C.keys, C.repr, C.sorted, x);
+    requires LC(C.k, C.next, C.prev, C.keys, C.repr, C.sorted, C.rev_sorted, x, alloc);
     requires x != null ==> C.sorted[x];
-    modifies Br, alloc, C.k, C.next, C.prev, C.keys, C.repr, C.sorted;
+    modifies Br, alloc, C.k, C.next, C.prev, C.keys, C.repr, C.sorted, C.rev_sorted;
+    ensures RefSetSubset(old(alloc), alloc);
     ensures ret != null;
-    ensures LC(C.k, C.next, C.prev, C.keys, C.repr, C.sorted, ret);
+    ensures LC(C.k, C.next, C.prev, C.keys, C.repr, C.sorted, C.rev_sorted, ret, alloc);
     ensures C.sorted[ret];
     ensures C.k[ret] == (if x != null && old(C.k)[x] <= k then old(C.k)[x] else k);
     ensures KeySetsEqual(C.keys[ret], (if x == null then EmptyKeySet else old(C.keys)[x])[k := true]);
-    ensures fresh(RefSetDiffF(C.repr[ret], (if x == null then EmptyRefSet else old(C.repr)[x])), alloc, old(alloc));
+    ensures Fresh(RefSetDiffF(C.repr[ret], (if x == null then EmptyRefSet else old(C.repr)[x])), alloc, old(alloc));
     ensures C.prev[ret] == null;
     ensures x != null ==> (ret == x || C.next[ret] == x);
     ensures (x == null || old(C.prev)[x] == null) ==> RefSetsEqual(Br, EmptyRefSet);
     ensures (x != null && old(C.prev)[x] != null) ==> RefSetsEqual(Br, EmptyRefSet[old(C.prev)[x] := true]);
+    // Framing conditions.
+    ensures Frame_all(C.k, C.next, C.prev, C.keys, C.repr, C.sorted, C.rev_sorted,
+                      old(C.k), old(C.next), old(C.prev), old(C.keys), old(C.repr), old(C.sorted), old(C.rev_sorted),
+                      if x == null then EmptyRefSet else old(C.repr)[x], old(alloc));
 {
     // Local variables
     var node: Ref;
     var tmp: Ref;
     var oldnext: Ref;
 
-    assume InAlloc(C.k, C.next, C.prev, C.keys, C.repr, C.sorted, x, alloc);
     if (x == null) {
         call node := Create(k);
         call Set_keys(node, EmptyKeySet[k := true]);
         call Set_repr(node, EmptyRefSet[node := true]);
         call Set_sorted(node, true);
+        call Set_rev_sorted(node, false);
 
         call AssertLCAndRemove(node);
 
@@ -59,6 +70,7 @@ procedure SortedListInsert(x: Ref, k: int) returns (ret: Ref)
         call Set_keys(node, (if C.next[node] == null then EmptyKeySet else C.keys[C.next[node]])[C.k[node] := true]);
         call Set_repr(node, (if C.next[node] == null then EmptyRefSet else C.repr[C.next[node]])[node := true]);
         call Set_sorted(node, true);
+        call Set_rev_sorted(node, false);
         call Set_prev(x, node);
 
         call AssertLCAndRemove(x);
@@ -68,7 +80,6 @@ procedure SortedListInsert(x: Ref, k: int) returns (ret: Ref)
     } else {
         if (C.next[x] != null) {
             call IfNotBr_ThenLC(C.next[x]);
-            assume InAlloc(C.k, C.next, C.prev, C.keys, C.repr, C.sorted, C.next[x], alloc);
         }
 
         call tmp := SortedListInsertContract(C.next[x], k);
